\documentclass{article}
\usepackage[utf8]{inputenc}
\usepackage{graphicx}
\usepackage{amsmath}
\usepackage{amsfonts}
\usepackage{amsbsy}
\usepackage{mathrsfs}
\usepackage{appendix}
\usepackage{amsthm}
\usepackage{bbold}
\usepackage{epstopdf}
\usepackage{stmaryrd}

\newcommand{\bs}[1]{\boldsymbol{#1}}
\newcommand{\bb}[1]{\mathbf{#1}}
\newcommand{\pd}[2]{\frac{\partial {#1}}{\partial {#2}}}
\newcommand{\parti}[1]{\pd{}{#1}}
\newcommand{\bigCI}{\mathrel{\text{\scalebox{1.07}{$\perp\mkern-10mu\perp$}}}}
\title{TP3 for Sub-pixel}
\author{Leman FENG\\ Email: flm8620@gmail.com\\Website: lemanfeng.com}

\begin{document}
	\maketitle
	\section{Ex 8}
	\subsection{1.}
	Let's firstly calculate Fourier transform of Dirac comb in 2D. Define Dirac comb with period $(T_1,T_2)$ as:
	
	\begin{equation}
	\Pi_{(T_1,T_2)} = \sum_{k,j\in \mathbb{Z}^2} \delta(x-jT_1,y-kT_2)
	\end{equation}
	
	Use Fourier series in 2d, $\Pi_{(T_1,T_2)}$ can be decomposed as:
	\begin{equation}
	\Pi_{(T_1,T_2)} = \sum_{k,j\in \mathbb{Z}^2} c_{j,k} \exp(i \frac{2j\pi}{T_1}x)  \exp(i \frac{2k\pi}{T_2}y)
	\end{equation}
	where
	\begin{equation}
	\begin{split}
	c_{j,k} &= \frac{1}{T_1T_2} \int_{-T_1/2}^{T_1/2} \int_{-T_2/2}^{T_2/2} \Pi_{(T_1,T_2)} \exp(-i\frac{2j\pi}{T_1}x)  \exp(-i\frac{2k\pi}{T_2}y) \\
	&= \frac{1}{T_1T_2} \langle \delta,\exp(-i\frac{2j\pi}{T_1}x)  \exp(-i\frac{2k\pi}{T_2}y)  \rangle\\
	&= \frac{1}{T_1T_2}
	\end{split}
	\end{equation}
	
	So we have 
	\begin{equation}
	\Pi_{(T_1,T_2)} = \frac{1}{T_1T_2} \sum_{k,j\in \mathbb{Z}^2} \exp(i \frac{2j\pi}{T_1}x)  \exp(i \frac{2k\pi}{T_2}y)
	\end{equation}
	
	Then we calculate $\hat{\Pi}_{(T_1,T_2)}$
	
	\begin{equation}
	\begin{split}
	\hat{\Pi}_{(T_1,T_2)} &= \iint \Pi_{(T_1,T_2)} \exp(-i \langle \begin{pmatrix}x\\y\end{pmatrix}, \begin{pmatrix}\xi_1\\\xi_2\end{pmatrix} \rangle) dxdy\\
	&= \langle \sum_{k,j\in \mathbb{Z}^2} \delta(x-jT_1,y-kT_2), \exp(-i \langle\begin{pmatrix}x\\y\end{pmatrix}, \begin{pmatrix}\xi_1\\\xi_2\end{pmatrix}\rangle) \rangle\\
	&= \sum_{k,j\in \mathbb{Z}^2} \exp(-ijT_1\xi_1) \exp(-ikT_2\xi_2)\\
	&= \sum_{k,j\in \mathbb{Z}^2} \exp(-i\frac{2j\pi}{s_1}\xi_1) \exp(-i\frac{2k\pi}{s_2}\xi_2)
	\end{split}
	\end{equation}
	where $s_1 = \frac{2\pi}{T_1}, s_2 = \frac{2\pi}{T_2}$, then we can rewrite
	\begin{equation}
	\hat{\Pi}_{(T_1,T_2)} = \frac{4\pi^2}{T_1T_2} \Pi_{(\frac{2\pi}{T_1},\frac{2\pi}{T_2})}
	\end{equation}
	
	Now define translation operator $\mathscr{T}^t$ in 2D:
	\begin{equation}
	\mathscr{T}^t(f)(x) = f(x-t)
	\end{equation}
	Fourier transform has property:
	\begin{equation}
	(\mathscr{F}\circ \mathscr{T}^t \circ f)(x) = \exp(-i\langle t,\xi\rangle) \hat{f}(\xi)
	\end{equation}
	
	\begin{equation}
	\begin{split}
	U &= \sum_{k\in \llbracket 0,M-1\rrbracket, l\in \llbracket 0,N-1\rrbracket } u[k,l] \sum_{m,n\in \mathbb{Z}^2} \delta_{(k+mM,l+nN)}\\
	&= \sum_{k,l } u[k,l] \mathscr{T}^{(k,l)}\circ\Pi_{(M,N)}\\
	\hat{U} &= \sum_{k,l} u[k,l]  \mathscr{F}\circ\mathscr{T}^{(k,l)}\Pi_{(M,N)}\\
	\hat{U} &= \sum_{k,l} u[k,l]  \exp(-i\langle (k,l),\xi\rangle)\hat{\Pi}_{(M,N)}\\
	\hat{U} &= \sum_{k,l} u[k,l]  \exp(-ik\xi_1) \exp(-il\xi_2) \frac{4\pi^2}{MN} \Pi_{(\frac{2\pi}{M},\frac{2\pi}{N})}\\
	\end{split}
	\end{equation}
	
	Notice that distribution can be multiplied by infinitely differentiable functions, so $\exp(-ik\xi_1) \exp(-il\xi_2) \frac{4\pi^2}{MN} \Pi_{(\frac{2\pi}{M},\frac{2\pi}{N})}$ make sense
	
	\begin{equation}
	\begin{split}
	\hat{U} &= \sum_{k,l} u[k,l]  \exp(-ik\xi_1) \exp(-il\xi_2) \frac{4\pi^2}{MN} \sum_{m,n\in \mathbb{Z}^2} \delta_{(\frac{2\pi}{M}m,\frac{2\pi}{N}n)}\\
	\hat{U} &=  \frac{4\pi^2}{MN} \sum_{k,l} u[k,l]  \sum_{m,n\in \mathbb{Z}^2} \delta_{(\frac{2\pi}{M}m,\frac{2\pi}{N}n)} \exp(-i\frac{2\pi m}{M}k) \exp(-i\frac{2\pi n}{N}l)\\
	\hat{U} &=  \frac{4\pi^2}{MN}  \sum_{m,n\in \mathbb{Z}^2}    \delta_{(\frac{2\pi}{M}m,\frac{2\pi}{N}n)} \sum_{k,l} u[k,l] \exp(-i\frac{2\pi k}{M}m) \exp(-i\frac{2\pi l}{N}n)\\
	\end{split}
	\end{equation}
	
	The DFT in 2D is defined as:
	\begin{equation}
	\hat{u}[p,q] = \sum_{k=0}^{M-1} \sum_{l=0}^{N-1} u[k,l] \exp(-i\frac{2\pi k}{M} p) \exp(-i\frac{2\pi l}{N} q), 0\leq p <M, 0 \leq q < N
	\end{equation}
	
	So
	\begin{equation}
	\begin{split}
	\hat{U} &=  \frac{4\pi^2}{MN}  \sum_{m,n\in \mathbb{Z}^2}    \delta_{(\frac{2\pi}{M}m,\frac{2\pi}{N}n)} \hat{u}[m\mod M,n \mod N]\\
	\hat{U} &=  \frac{4\pi^2}{MN}  \sum_{k=0}^{M-1} \sum_{l=0}^{N-1} \hat{u}[k,l] \sum_{m,n\in \mathbb{Z}^2} \delta_{(\frac{2\pi k}{M}+2\pi m,\frac{2\pi l}{N}+2 \pi n)}\\
	\end{split}
	\end{equation}
\end{document}
